correction to def resultSet (**) with sel contribSet
Agents now only observe the contribSet of the other call participant
and not their own contribSet as before, which could make them see
their own transmission mistakes.

The proof of `indistinguishable_then_same_values` also seems doable
now, though only 2 out of 18 cases are done.

Gossip/Error/SyncCorrection.lean
@@ -1,5 +1,6 @@
 import Mathlib.Data.Set.Basic
 import Mathlib.Data.Prod.Basic
+import Mathlib.Tactic.DepRewrite
 import Mathlib.Tactic.Linarith
 
 namespace Error
@@ -98,6 +99,8 @@ def Form.length : @Form n → Nat
   | S _ _ => 1
   | K _ φ => 1 + φ.length
 
+/-! ## Roles -/
+
 inductive Role : Type
   | Caller : Role
   | Callee : Role
@@ -160,25 +163,26 @@ def resultSet (i : @Agent n) : @Dist n → @Sequence n → Set (@Value n)
   | ι, (C :: σ) =>
     /- (*) Values that `i` already knows to be wrong before the call (and can thus refuse). -/
     let refuse : Set Value := { ⟨j, d⟩ | eval ι σ (K i (S j (j, !d))) }
-    /- (**) Values that `i` knows to be wrong after the call (and can thus delete). -/
-    let delete : Set Value := { ⟨j, d⟩ | ∀ ι' τ D, equiv i (ι,⟨σ,rfl⟩) (ι',τ)
+    /- (**) Values that `i` knows to be wrong after the call (and can thus delete).
+    The `sel` here decides which part of `contribSet` agent `a` may see (namely: not its own). -/
+    let delete sel : Set Value := { ⟨j, d⟩ | ∀ ι' τ D, equiv i (ι,⟨σ,rfl⟩) (ι',τ)
                                 -- paper: → resultSet (other i C) ι' σ = resultSet (other i C) ι' τ
                                 -- new version here also allowing other calls:
                                           → roleOfIn i C = roleOfIn i D
-                                          → contribSet ι σ C = contribSet ι' τ D
+                                          → sel (contribSet ι σ C) = sel (contribSet ι' τ D)
                                           → eval ι' τ (S j (j, !d)) }
     match C, roleOfIn i C with
       -- Not involved:
       | _, Other => resultSet i ι σ
       -- Normal calls
-      | ⌜ a b ⌝, Caller => ((resultSet a ι σ ∪ resultSet b ι σ) \ refuse) \ delete
-      | ⌜ a b ⌝, Callee => ((resultSet a ι σ ∪ resultSet b ι σ) \ refuse) \ delete
+      | ⌜ a b ⌝, Caller => ((resultSet a ι σ ∪ resultSet b ι σ) \ refuse) \ delete Prod.snd
+      | ⌜ a b ⌝, Callee => ((resultSet a ι σ ∪ resultSet b ι σ) \ refuse) \ delete Prod.fst
       -- error from a (but not for a itself)
-      | ⌜ a^_ b ⌝, Caller => ((          resultSet a ι σ  ∪ resultSet b ι σ) \ refuse) \ delete
-      | ⌜ a^c b ⌝, Callee => ((invert c (resultSet a ι σ) ∪ resultSet b ι σ) \ refuse) \ delete
+      | ⌜ a^_ b ⌝, Caller => ((          resultSet a ι σ  ∪ resultSet b ι σ) \ refuse) \ delete Prod.snd
+      | ⌜ a^c b ⌝, Callee => ((invert c (resultSet a ι σ) ∪ resultSet b ι σ) \ refuse) \ delete Prod.fst
       -- error from b (but not for b itself)
-      | ⌜ a b^c ⌝, Caller => ((resultSet a ι σ ∪ invert c (resultSet b ι σ)) \ refuse) \ delete
-      | ⌜ a b^_ ⌝, Callee => ((resultSet a ι σ ∪           resultSet b ι σ ) \ refuse) \ delete
+      | ⌜ a b^c ⌝, Caller => ((resultSet a ι σ ∪ invert c (resultSet b ι σ)) \ refuse) \ delete Prod.snd
+      | ⌜ a b^_ ⌝, Callee => ((resultSet a ι σ ∪           resultSet b ι σ ) \ refuse) \ delete Prod.fst
 termination_by
   _ σ => (σ.length, 0) -- should be below contribSet
 decreasing_by
@@ -464,89 +468,107 @@ lemma equiv_then_know_same {a m ι} {σ : @Sequence n} {h1 : σ.length = m} {κ 
     convert this
 
 /-- Lemma 7 -/
-lemma indistinguishable_then_same_values {ι ι': Dist} {σ k : Sequence} :
-    (ι, σ) ~_a (ι', k)  →  ι⌈σ⌉a = ι'⌈k⌉a := by
+lemma indistinguishable_then_same_values {n} {a : @Agent n} {ι ι': @Dist n} {σ τ : Sequence} :
+    (ι, σ) ~_a (ι', τ)  →  ι⌈σ⌉a = ι'⌈τ⌉a := by
   intro ⟨same_len, equ⟩
   simp at same_len
-  induction σ generalizing k
+  induction σ generalizing τ
   case nil =>
     have := List.length_eq_zero_iff.mp same_len.symm
     aesop
-  case cons C σ' IH =>
+  case cons C σ IH =>
     simp at same_len
-    rcases List.exists_cons_of_length_eq_add_one same_len.symm with ⟨Cτ, τ', τ_def⟩
-    subst τ_def
+    rcases List.exists_cons_of_length_eq_add_one same_len.symm with ⟨D, τ, _def⟩
+    subst _def
     simp only [List.length_cons, equiv, Nat.add_one_sub_one] at equ
-    specialize IH (by grind) equ.1 -- IH now says `ι⌈σ'⌉a = ι'⌈τ'⌉a`
-    -- distinguish cases whether a is involved in κ (and this also κ') or not
+    specialize IH (by grind) equ.1 -- IH now says `ι⌈σ⌉a = ι'⌈τ⌉a`
+    -- distinguish cases whether/how a is involved in C (and thus also D) or not
     cases r : roleOfIn a C
-    case Caller =>
+    case Caller => -- first out of three outer cases
       simp [r] at equ
       rcases equ with ⟨prev_equ, Caller_eq, prev_same_contrib, same_pair⟩
       unfold contribSet at prev_same_contrib
       let C_copy := C
-      cases C <;> cases Cτ <;> simp [Call.pair, roleOfIn_eq_Caller_iff] at *
-      case normal.normal =>
+      cases C <;> cases D <;> simp [Call.pair, roleOfIn_eq_Caller_iff] at *
+      all_goals
         rcases same_pair with ⟨_,_⟩
         subst_eqs
-        simp at same_len
+        simp only [List.length_cons, Nat.add_right_cancel_iff] at same_len
         clear Caller_eq
+      case normal.normal => -- 1 of 9 subcases
+        simp only [roleOfIn_a, resultSet]
         ext ⟨d,k⟩
-        -- rw [IH] -- probaly not enough use of IH here?
-        simp [resultSet, contribSet, eval]
         constructor
-          <;> rintro ⟨⟨dk_in, h22⟩, ⟨ι2, σ2, ⟨⟨σ2_len, σ'_equiv_σ2⟩, ⟨C, same_role, def_contrib, ndk_in⟩⟩⟩⟩
+        all_goals
+          intro dk_in
+          simp only [Subtype.forall, Set.mem_diff, Set.mem_union, Set.mem_setOf_eq] at dk_in
+          rcases dk_in with ⟨⟨someone_had_dk_before, dk_not_refused⟩, not_self_corrected⟩
         · refine ⟨⟨?_, ?_⟩, ?_⟩
-          · rw [← IH]
-            simp_all
-          · use ι2, σ2
-            simp_all
-            apply @equiv_trans _ a _ ι' τ' rfl ι σ' same_len ι2 σ2
-            · apply equiv_of_equi
-              apply equi_of_equiv
-              exact equiv_symm.mpr prev_equ
-            · apply equiv_of_equi
-              apply equi_of_equiv
-              exact σ'_equiv_σ2
-          · use ι2, σ2
-            simp_all
-            constructor
-            · apply @equiv_trans _ a _ ι' τ' rfl ι σ' same_len ι2 σ2
-              · apply equiv_of_equi
-                apply equi_of_equiv
-                exact equiv_symm.mpr prev_equ
-              · apply equiv_of_equi
-                apply equi_of_equiv
-                exact σ'_equiv_σ2
-            · sorry -- unclear here
-        · sorry
+          · rw [← IH]; simp_all
+          · rw [Set.mem_setOf_eq, ← equiv_then_know_same prev_equ]; exact dk_not_refused
+          · simp -- FIXME `simp only` does too little here
+            simp at not_self_corrected -- `a` considers a state that justifies keeping (d,k)
+            rcases not_self_corrected with ⟨ι2, σ2, ⟨len2, equ2⟩, ⟨C2, role2, same_contrib_2, ndk⟩⟩
+            refine ⟨ι2, σ2, ⟨by omega, ?_⟩, C2, role2, ?_, ndk⟩
+            · have := equiv_trans (equiv_symm.mp prev_equ) equ2; rw! [same_len] at *; exact this
+            · grind [contribSet]
+        · refine ⟨⟨?_, ?_⟩, ?_⟩ -- adapted copy-pasta
+          · rw [IH]; simp_all
+          · rw [Set.mem_setOf_eq, equiv_then_know_same prev_equ]; exact dk_not_refused
+          · simp -- FIXME `simp only` does too little here
+            simp at not_self_corrected -- `a` considers a state that justifies keeping (d,k)
+            rcases not_self_corrected with ⟨ι2, σ2, ⟨len2, equ2⟩, ⟨C2, role2, same_contrib_2, ndk⟩⟩
+            refine ⟨ι2, σ2, ⟨by omega, ?_⟩, C2, role2, ?_, ndk⟩
+            · apply equiv_trans prev_equ; rw! [same_len]; exact equ2
+            · grind [contribSet]
+      case normal.fstE =>
+        simp only [roleOfIn_a, resultSet, Subtype.forall, roleOfIn_fstE_eq_Caller_iff]
+        ext ⟨d,k⟩
+        constructor
+        · intro dk_in
+          simp only [Set.mem_diff, Set.mem_union, Set.mem_setOf_eq, not_forall] at dk_in
+          rcases dk_in with ⟨⟨someone_had_dk_before, dk_not_refused⟩, not_self_corrected⟩
+          refine ⟨⟨?_, ?_⟩, ?_⟩
+          · rw [← IH]; simp_all
+          · rw [Set.mem_setOf_eq, ← equiv_then_know_same prev_equ]; exact dk_not_refused
+          · simp -- FIXME `simp only` does too little here
+            simp at not_self_corrected -- `a` considers a state that justifies keeping (d,k)
+            rcases not_self_corrected with ⟨ι2, σ2, len2, C2, same_contrib_2, role2, equ2, ndk⟩
+            refine ⟨ι2, σ2, ⟨by omega, ?_⟩, C2, ?_, ?_, ndk⟩
+            · have := equiv_trans (equiv_symm.mp prev_equ) equ2; rw! [same_len] at *; exact this
+            · rw [← role2]; simp
+            · simp [contribSet] -- here the `sel` in `resultSet` matters
+              rw [← prev_same_contrib]
+              rw [← same_contrib_2]
+              simp [contribSet]
+        · -- todo copy pasta adaptation
+          sorry
+      case normal.sndE =>
+        sorry
 
-      all_goals
-        rcases same_pair with ⟨_,_⟩
-        subst_eqs
-        simp at same_len
-        clear Caller_eq
-        simp [resultSet]
-        sorry -- grind [equiv_then_know_same, roleOfIn_a]
+      case fstE.normal =>
+        sorry
+      case fstE.fstE =>
+        sorry
+      case fstE.sndE =>
+        sorry
+
+      case sndE.normal =>
+        sorry
+      case sndE.fstE =>
+        sorry
+      case sndE.sndE =>
+        sorry
+
     case Callee =>
-      simp [r] at equ
-      rcases equ with ⟨prev_equ, Callee_eq, prev_same_contrib, same_pair⟩
-      unfold contribSet at prev_same_contrib
-      cases C <;> cases Cτ <;> simp [Call.pair, roleOfIn_eq_Callee_iff] at *
-        <;> rcases r with ⟨not_a, h⟩ <;> subst h
-      all_goals
-        rcases same_pair with ⟨_,_⟩
-        subst_eqs
-        simp at same_len
-        clear Callee_eq
-        simp [resultSet, not_a]
-        sorry -- grind [equiv_then_know_same, roleOfIn_a]
+      -- Should be similar to `Caller` cases.
+      sorry
     case Other =>
       unfold resultSet
       rw [r]
       rw [equ.2.1] at r
       rw [r]
-      simp
+      simp only
       exact IH
 
 /-- Lemma 8. The truth value of any "a has ..." atom is known by a.
@@ -560,6 +582,8 @@ lemma local_is_known {a b : @Agent n} (k : Bool) :
     intro ι σ bk_in κ τ same_len equ
     have := indistinguishable_then_same_values ⟨?_, equ⟩ -- using Lemma 7
     <;> grind
+
+/-! NOTE: the remaining lemmas do not use Lemma 7 and 8, better reorder them later? -/
 
 /-- Helper for Lemma 9, stronger version using a specific `k` and not `Kv`. -/
 lemma knowledge_of_secrets_is_preserved' {a b : Agent} (k : Bool)
